AP/System/Invariant.lean
@@ -5,25 +5,27 @@ namespace System
 universe u
 variable {S T : Type u} {sys : System S T}
 
-theorem invariant {p : S → Prop} {a b}
+theorem invariant {p : S → Prop} {a b} [ha : sys.WF a]
 (h₁ : p a) (h₂ : sys.Reachable a b)
-(h₃ : ∀ {x y t}, p x → sys.tr x t = some y → p y) : p b := by
-  induction h₂; exact h₁
-  clear a b
+(h₃ : ∀ {x y t} [sys.WF x] [sys.WF y], p x → sys.tr x t = some y → p y) : p b := by
+  revert ha; induction h₂; exact h₁
+  clear! a b
   nm a b c t h₂ h₄ ih
+  intro ha
+  have hb := wf_of_tr h₂
   apply ih
   exact h₃ h₁ h₂
 
-theorem invariant_init {p : S → Prop} {a}
+theorem invariant_wf {p : S → Prop} {a}
 (h₁ : sys.WF a) (h₂ : ∀ {a}, sys.Initial a → p a)
-(h₃ : ∀ {x y t}, p x → sys.tr x t = some y → p y) : p a := by
+(h₃ : ∀ {x y t} [sys.WF x] [sys.WF y], p x → sys.tr x t = some y → p y) : p a := by
   rw [wf_def] at h₁
   obtain ⟨s₀, h₁, h₄⟩ := h₁
   exact invariant (h₂ h₁) h₄ h₃
 
-theorem invariant_val {α : Type*} {a b} {f : S → α} (h₁ : sys.Reachable a b)
-(h₂ : ∀ {x y t}, sys.tr x t = some y → f y = f x) : f b = f a := by
+theorem invariant_val {α : Type*} {a b} [ha : sys.WF a] {f : S → α} (h₁ : sys.Reachable a b)
+(h₂ : ∀ {x y t} [sys.WF x] [sys.WF y], sys.tr x t = some y → f y = f x) : f b = f a := by
   apply invariant (p := (f · = f a)) rfl h₁
-  intro x y t h₃ h₄
+  intro x y t ha hb h₃ h₄
   rw [←h₃]
   exact h₂ h₄
